<a id="readme-top"></a> 

- [Precalculus](#precalculus)
  - [Evaluate Powers of ( i )](#evaluate-powers-of--i-)
  - [Substitute Values into the Expression](#substitute-values-into-the-expression)
  - [Group Real and Imaginary Terms](#group-real-and-imaginary-terms)
  - [Find ( a + b )](#find--a--b-)
  - [Final Answer](#final-answer)
  - [How to Solve Similar Problems Faster?](#how-to-solve-similar-problems-faster)
- [Radian](#radian)
  - [Solving the Equation: ( \\sin x = \\cos y )](#solving-the-equation--sin-x--cos-y-)
  - [Step 1: Recognize the Identity](#step-1-recognize-the-identity)
  - [Step 2: Apply the Identity](#step-2-apply-the-identity)
  - [Step 3: Solve for ( x )](#step-3-solve-for--x-)
  - [Step 4: Verify the Answer](#step-4-verify-the-answer)
  - [How the Identity Works:](#how-the-identity-works)
  - [Example:](#example)
  - [How This Helps Solve Similar Problems:](#how-this-helps-solve-similar-problems)
  - [Helpful YouTube Video](#helpful-youtube-video)

---
# Precalculus

## Evaluate Powers of \( i \)
Since \( i = \sqrt{-1} \), the powers of \( i \) follow a repeating cycle:

\[
i^1 = i, \quad i^2 = -1, \quad i^3 = -i, \quad i^4 = 1, \quad i^5 = i, \quad \dots
\]

---

## Substitute Values into the Expression
Given:

\[
2 + 3i + 4i^2 + 5i^3 + 6i^4
\]

Using the cycle:

- \( i^2 = -1 \Rightarrow 4i^2 = 4(-1) = -4 \)
- \( i^3 = -i \Rightarrow 5i^3 = 5(-i) = -5i \)
- \( i^4 = 1 \Rightarrow 6i^4 = 6(1) = 6 \)

Rewriting the expression:

\[
2 + 3i - 4 - 5i + 6
\]

---

## Group Real and Imaginary Terms
Real terms:

\[
2 - 4 + 6 = 4
\]

Imaginary terms:

\[
3i - 5i = -2i
\]

Thus, the expression simplifies to:

\[
4 - 2i
\]

---

## Find \( a + b \)
Since \( a = 4 \) and \( b = -2 \),

\[
a + b = 4 + (-2) = 2
\]

---

## Final Answer
\[
\boxed{2}
\]


---

## How to Solve Similar Problems Faster?
- **Memorize the cycle of \( i \):**
  \[
  i^1 = i, \quad i^2 = -1, \quad i^3 = -i, \quad i^4 = 1
  \]
  (Repeats every 4 steps.)

- **Substitute values for \( i^n \) quickly.**

- **Group real and imaginary parts.**

- **Simplify.**

---

# Radian

## Solving the Equation: \( \sin x = \cos y \)

We are given the equation:

\[
\sin x = \cos y
\]

and we want to solve for \( x \) in terms of \( y \).

---

## Step 1: Recognize the Identity

We use the fundamental trigonometric identity:

\[
\sin \left( \frac{\pi}{2} - \theta \right) = \cos \theta
\]

This identity tells us that the sine of \( \frac{\pi}{2} - \theta \) is equal to the cosine of \( \theta \). We can apply this identity to our equation.

---

## Step 2: Apply the Identity

We are given \( \sin x = \cos y \). Using the identity, we know that:

\[
\sin \left( \frac{\pi}{2} - y \right) = \cos y
\]

So, we can rewrite the equation as:

\[
\sin x = \sin \left( \frac{\pi}{2} - y \right)
\]

---

## Step 3: Solve for \( x \)

From the equation \( \sin x = \sin \left( \frac{\pi}{2} - y \right) \), we know that the sine function is one-to-one between \( 0 \) and \( \pi \). Therefore, we can directly set:

\[
x = \frac{\pi}{2} - y
\]

---

## Step 4: Verify the Answer

Now, letâ€™s check the options provided:

- \( \frac{\pi}{2} - y \)
- \( \frac{\pi}{2} + y \)
- \( y - \frac{\pi}{2} \)
- \( \pi - y \)

The correct choice is **\( \frac{\pi}{2} - y \)**, which matches the result we derived.

---

## How the Identity Works:

- The identity \( \sin \left( \frac{\pi}{2} - \theta \right) = \cos \theta \) helps us understand the relationship between sine and cosine functions for complementary angles. 
- In the unit circle, the sine of an angle \( \frac{\pi}{2} - \theta \) is equal to the cosine of the original angle \( \theta \). This identity is a fundamental relationship that allows us to switch between sine and cosine when the angles are complementary.
  
---

## Example:

If \( \theta = 30^\circ \) (or \( \frac{\pi}{6} \) radians):

- \( \sin \left( \frac{\pi}{2} - \frac{\pi}{6} \right) = \sin \frac{\pi}{3} = \frac{\sqrt{3}}{2} \)
- \( \cos \frac{\pi}{6} = \frac{\sqrt{3}}{2} \)

This shows that \( \sin \left( \frac{\pi}{2} - \theta \right) = \cos \theta \), confirming the identity.

---

## How This Helps Solve Similar Problems:

1. **Identify the identity:** Recognize when an equation involves \( \sin \) and \( \cos \), and use the identity \( \sin \left( \frac{\pi}{2} - \theta \right) = \cos \theta \).
2. **Rewrite the equation:** If you have an equation like \( \sin x = \cos y \), rewrite it as \( \sin x = \sin \left( \frac{\pi}{2} - y \right) \).
3. **Solve for the unknown variable:** From \( \sin x = \sin \left( \frac{\pi}{2} - y \right) \), solve for \( x \), which gives \( x = \frac{\pi}{2} - y \).
4. **Verify with options:** If given multiple choices, check which one matches the derived result.
## Helpful YouTube Video

For a more detailed explanation of trigonometric identities, you can watch this video on **trigonometric identities and solving equations**:

- [Trigonometric Identities: Sine, Cosine, and Tangent](https://www.youtube.com/watch?v=PUB0TaZ7bhA)
- [Trigonometric Equations Explained](https://www.youtube.com/watch?v=m1OitPmkydY)


---



<p align="right">(<a href="#readme-top">back to top</a>)</p>


<br /><br /><br />